clarified context;

thys/Automatic_Refinement/Lib/Indep_Vars.thy
@@ -7,26 +7,25 @@ lemma INDEPI: "INDEP v" by simp
 
 ML {*
   signature INDEP_VARS = sig
-    val indep_tac: tactic'
+    val indep_tac: Proof.context -> tactic'
   end
 
-  structure Indep_Vars :INDEP_VARS = struct
+  structure Indep_Vars: INDEP_VARS = struct
 
     local
       fun vsubterms (Abs (_,_,t)) = vsubterms t
         | vsubterms (t as (_$_)) = let
             val (f,args) = strip_comb t
             val args_vsts = map vsubterms args |> flat
-          in 
-            case f of 
+          in
+            case f of
               (Var (name,vT)) => [(name,vT,fastype_of t,args)]@args_vsts
             | _ => vsubterms f @ args_vsts
           end
         | vsubterms _ = []
 
-      fun indep_vars t st = let
-        val thy = Thm.theory_of_thm st
-        val cert = Thm.global_cterm_of thy
+      fun indep_vars ctxt t st = let
+        val cert = Thm.cterm_of ctxt
 
         fun inst_of (name,vT,T,args) = let
           val Ts = map fastype_of args |> rev
@@ -40,109 +39,21 @@ ML {*
 
         val st' = Drule.instantiate_normalize ([],inst) st
           |> Conv.fconv_rule (Thm.beta_conversion true)
-      in 
-        Seq.single st' 
+      in
+        Seq.single st'
       end
-      
-      fun indep_tac_aux i st = case Logic.concl_of_goal (Thm.prop_of st) i of
-        @{mpat "Trueprop (INDEP ?v)"} 
-          => (indep_vars v THEN rtac @{thm INDEPI} i) st
+
+      fun indep_tac_aux ctxt i st = case Logic.concl_of_goal (Thm.prop_of st) i of
+        @{mpat "Trueprop (INDEP ?v)"}
+          => (indep_vars ctxt v THEN rtac @{thm INDEPI} i) st
       | _ => Seq.empty
 
     in
       (* Remove explicit parameters from schematic variable. *)
-      val indep_tac = IF_EXGOAL 
-        (CONVERSION Thm.eta_conversion THEN' indep_tac_aux)
+      fun indep_tac ctxt = IF_EXGOAL
+        (CONVERSION Thm.eta_conversion THEN' indep_tac_aux ctxt)
     end
   end
 *}
 
-
-(*schematic_lemma 
-  "!!x y z. INDEP (?R x z)"
-  "!!x y z. ?R x z 1"
-  apply (tactic {* Indep_Vars.indep_tac 1 *})
-  apply rule
-  done
-*)
-
-
-
 end
-
-(*
-
-      fun indep_vars t st = case strip_comb t of
-        (v as Var (name,_),args) => let
-          val thy = theory_of_thm st
-          val cert = Thm.global_cterm_of thy
-  
-          val T = fastype_of t
-          val Ts = map fastype_of args |> rev
-          val t' = fold absdummy Ts (Var (name,T))
-          val inst = ([],[(cert v, cert t')]) handle e =>
-            ( tracing (Syntax.pretty_term_global thy t |> Pretty.string_of);
-              reraise e
-            )
-
-          val st' = Drule.instantiate_normalize inst st
-            |> Conv.fconv_rule (Thm.beta_conversion true)
-
-          val _ = Config.get_global thy cfg_trace andalso (Pretty.block [
-            Pretty.str "INDEP ", Syntax.pretty_term_global thy t, 
-              Pretty.brk 1, Pretty.str ":", Pretty.brk 1,
-              Syntax.pretty_term_global thy v,
-              Pretty.brk 1, Pretty.str "->", Pretty.brk 1,
-              Syntax.pretty_term_global thy t',
-              Pretty.fbrk,
-              Pretty.indent 2 (
-                Pretty.big_list "Goals: " 
-                  (Goal_Display.pretty_goals_without_context st'))
-          ] |> Pretty.string_of |> tracing; true)
-
-        in Seq.single st' end
-      | _ => (
-        Pretty.block [ 
-            Pretty.str "INDEP on non-variable: ", 
-            Syntax.pretty_term_global (theory_of_thm st) t
-          ] |> Pretty.string_of |> warning;
-        Seq.single st
-      )
-
-
-
-  Old version: Removes all functionality, not only explicit parameters
-  structure Indep_Vars :INDEP_VARS = struct
-    local
-      (* Remove explicit parameters from relation variable. *)
-      fun indep_var (name,typ) = let
-        val (Ts,T) = strip_type typ |>> rev
-        val r = fold absdummy Ts (Var (name,T))
-      in 
-        r
-      end
-
-      fun indep_vars R st = let
-        val vs = Term.add_vars R []
-        val cert = Thm.global_cterm_of (theory_of_thm st)
-        val inst = map (fn v => (cert (Var v), cert (indep_var v))) vs
-        val st' = Drule.instantiate_normalize ([],inst) st
-          |> Conv.fconv_rule (Thm.beta_conversion true)
-      in 
-        Seq.single st'
-      end
-
-      fun indep_tac_aux i st = case Logic.concl_of_goal (prop_of st) i of
-        @{mpat "Trueprop (INDEP ?v)"} 
-          => (indep_vars v THEN rtac @{thm INDEPI} i) st
-      | _ => Seq.empty
-
-    in
-      val indep_tac = IF_EXGOAL indep_tac_aux
-
-    end
-  end
-
-
-
-*)
