thys/Automatic_Refinement/Tool/Autoref_Fix_Rel.thy
@@ -99,9 +99,9 @@ ML {*
     val constraints_of_goal: int -> thm -> (term * term) list
 
     val mk_CONSTRAINT: term * term -> term 
-    val mk_CONSTRAINT_rl: theory -> constraint -> thm
+    val mk_CONSTRAINT_rl: Proof.context -> constraint -> thm
 
-    val insert_CONSTRAINTS_tac: tactic'
+    val insert_CONSTRAINTS_tac: Proof.context -> tactic'
 
     val constraint_of_thm: thm -> constraint
 
@@ -128,7 +128,7 @@ ML {*
     val get_tyrel_rules: Proof.context -> thm list
 
 
-    val insert_tyrel_tac : int -> int -> tactic'
+    val insert_tyrel_tac : Proof.context -> int -> int -> tactic'
     val solve_tyrel_tac : Proof.context -> tactic'
     val tyrel_tac : Proof.context -> itactic
 
@@ -209,19 +209,19 @@ ML {*
     end;
 
     (* Types of f and R must match! *)
-    fun mk_CONSTRAINT_rl thy (ps,c) = let
+    fun mk_CONSTRAINT_rl ctxt (ps,c) = let
       val ps = map (mk_CONSTRAINT #> HOLogic.mk_Trueprop) ps
       val c = mk_CONSTRAINT c |> HOLogic.mk_Trueprop
       val g = Logic.list_implies (ps,c)
-      val thm = Goal.prove_global thy [] [] g (K (rtac @{thm CONSTRAINTI} 1)) 
-    in 
-      thm
+    in
+      (* FIXME use proper context *)
+      Goal.prove_global (Proof_Context.theory_of ctxt) [] [] g (K (rtac @{thm CONSTRAINTI} 1))
     end;
 
     (* Internal use for hom-patterns, f and R are unified *)
-    fun mk_CONSTRAINT_rl_atom thy (f,R) = let
+    fun mk_CONSTRAINT_rl_atom ctxt (f,R) = let
       open Refine_Util
-      val ts = map (SOME o Thm.global_cterm_of thy) [f,R]
+      val ts = map (SOME o Thm.cterm_of ctxt) [f,R]
       val idx = Term.maxidx_term f (Term.maxidx_of_term R) + 1
       val thm = cterm_instantiate' ts 
         (Thm.incr_indexes idx @{thm CONSTRAINTI})
@@ -229,10 +229,9 @@ ML {*
       thm
     end;
 
-    fun insert_CONSTRAINTS_tac i st = let
-      val thy = Thm.theory_of_thm st
+    fun insert_CONSTRAINTS_tac ctxt i st = let
       val cs = constraints_of_goal i st 
-      |> map (mk_CONSTRAINT #> HOLogic.mk_Trueprop #> Thm.global_cterm_of thy)
+      |> map (mk_CONSTRAINT #> HOLogic.mk_Trueprop #> Thm.cterm_of ctxt)
     in
       Refine_Util.insert_subgoals_tac cs i st
     end
@@ -510,8 +509,7 @@ ML {*
       fun compute_hom_net pairs ctxt = let
         val cs = map_filter #1 pairs
         val cs' = map (fn (_,(f,R)) => (f,hom_pat_of_rel ctxt R)) cs
-        val thy = Proof_Context.theory_of ctxt
-        val thms = get_hom_rules ctxt @ map (mk_CONSTRAINT_rl_atom thy) cs'
+        val thms = get_hom_rules ctxt @ map (mk_CONSTRAINT_rl_atom ctxt) cs'
         val thms = map (Thm.cprop_of #> Thm.trivial) thms
         val net = Tactic.build_net thms
       in
@@ -567,14 +565,12 @@ ML {*
   
     in
 
-      fun insert_tyrel_tac i j k st = let
-        val thy = Thm.theory_of_thm st
-
+      fun insert_tyrel_tac ctxt i j k st = let
         fun get_constraint t = let
           val T = fastype_of t
           val res = Const (@{const_name TYREL}, T --> HOLogic.boolT) $ t
         in
-          res |> HOLogic.mk_Trueprop |> Thm.global_cterm_of thy
+          res |> HOLogic.mk_Trueprop |> Thm.cterm_of ctxt
         end
         
         val relators = fold (add_relators_of_subgoal st) (i upto j) []
@@ -595,7 +591,7 @@ ML {*
     end
     
     fun tyrel_tac ctxt i j =
-      (insert_tyrel_tac i j
+      (insert_tyrel_tac ctxt i j
       THEN_ALL_NEW_FWD solve_tyrel_tac ctxt) i
 
 
@@ -608,13 +604,12 @@ ML {*
 
     fun internal_spec_tac ctxt = let
       val pairs = thm_pairsD.get ctxt
-      val thy = Proof_Context.theory_of ctxt
       val net = pairs
-        |> map_filter (fst #> map_option (snd #> mk_CONSTRAINT_rl_atom thy))
+        |> map_filter (fst #> map_option (snd #> mk_CONSTRAINT_rl_atom ctxt))
         |> Tactic.build_net
     in 
       fn i => fn j => REPEAT (CHANGED 
-        (Seq.INTERVAL (DETERM o Anti_Unification.specialize_net_tac net) i j)
+        (Seq.INTERVAL (DETERM o Anti_Unification.specialize_net_tac ctxt net) i j)
       )
     end
 
@@ -630,9 +625,8 @@ ML {*
 
     fun internal_solve_tac ctxt = let
       val pairs = thm_pairsD.get ctxt
-      val thy = Proof_Context.theory_of ctxt
       val net = pairs
-        |> map_filter (fst #> map_option (mk_CONSTRAINT_rl thy))
+        |> map_filter (fst #> map_option (mk_CONSTRAINT_rl ctxt))
         |> Tactic.build_net
 
       val s_tac = SOLVED' (REPEAT_ALL_NEW (resolve_from_net_tac ctxt net))
@@ -644,9 +638,8 @@ ML {*
 
     fun guess_relators_tac ctxt = let
       val pairs = thm_pairsD.get ctxt
-      val thy = Proof_Context.theory_of ctxt
       val net = pairs
-        |> map_filter (fst #> map_option (mk_CONSTRAINT_rl thy))
+        |> map_filter (fst #> map_option (mk_CONSTRAINT_rl ctxt))
         |> Tactic.build_net
 
       val hom_net = hom_netD.get ctxt
@@ -656,7 +649,7 @@ ML {*
 
       fun spec_tac i j = 
         REPEAT (CHANGED 
-          (Seq.INTERVAL (DETERM o Anti_Unification.specialize_net_tac net) i j)
+          (Seq.INTERVAL (DETERM o Anti_Unification.specialize_net_tac ctxt net) i j)
         )
 
       val solve_tac = let 
@@ -667,7 +660,7 @@ ML {*
         apply_to_constraints (TRY o DETERM o s_tac)
       end
     in
-      Seq.INTERVAL insert_CONSTRAINTS_tac
+      Seq.INTERVAL (insert_CONSTRAINTS_tac ctxt)
       THEN_INTERVAL hom_tac
       THEN_INTERVAL spec_tac
       THEN_INTERVAL (tyrel_tac ctxt)
@@ -713,13 +706,13 @@ ML {*
       (map (pretty_thm_pair ctxt) pairs)
 
     local
-      fun unifies thy (t1,t2) = Term.could_unify (t1,t2) andalso
+      fun unifies ctxt (t1, t2) = Term.could_unify (t1, t2) andalso
         let
           val idx1 = Term.maxidx_of_term t1
           val t2 = Logic.incr_indexes ([], [], idx1 + 1) t2
           val idx2 = Term.maxidx_of_term t2
         in
-          can (Pattern.unify (Context.Theory thy) (t1,t2)) (Envir.empty idx2)
+          can (Pattern.unify (Context.Proof ctxt) (t1,t2)) (Envir.empty idx2)
         end
 
       fun analyze_possible_problems ctxt (f,R) = let
@@ -817,7 +810,6 @@ ML {*
           @{mpat "Trueprop (CONSTRAINT ?f ?R)"} =>
             let
               val pairs = thm_pairsD.get ctxt
-              val thy = Proof_Context.theory_of ctxt
               val st = Drule.zero_var_indexes st
 
               val pt_hd = Pretty.block [
@@ -826,7 +818,7 @@ ML {*
               ]
 
               fun isc (SOME (ps,(fp,R)),_) = 
-                    if unifies thy (f,fp) then SOME (ps,(fp,R)) else NONE
+                    if unifies ctxt (f,fp) then SOME (ps,(fp,R)) else NONE
                 | isc _ = NONE
 
               val candidates = pairs |> map_filter isc
@@ -837,7 +829,7 @@ ML {*
                   pretty_constraint ctxt c
                 ]
 
-                val rl = mk_CONSTRAINT_rl thy c 
+                val rl = mk_CONSTRAINT_rl ctxt c 
                    |> Drule.zero_var_indexes
                 val res = (SOLVED' (rtac rl)) i st
                   |> Seq.pull |> is_some
@@ -911,7 +903,6 @@ ML {*
             @{mpat "Trueprop (CONSTRAINT ?f ?R)"} =>
               let
                 val pairs = thm_pairsD.get ctxt
-                val thy = Proof_Context.theory_of ctxt
                 val st = Drule.zero_var_indexes st
 
                 val pt = Pretty.block [
@@ -925,11 +916,11 @@ ML {*
                 | SOME p => tracing (Pretty.string_of p)
             
                 fun isc (SOME (ps,(fp,R)),_) = 
-                      if unifies thy (f,fp) then SOME (ps,(fp,R)) else NONE
+                      if unifies ctxt (f,fp) then SOME (ps,(fp,R)) else NONE
                   | isc _ = NONE
 
                 val net = pairs
-                  |> map_filter (fst #> map_option (mk_CONSTRAINT_rl thy))
+                  |> map_filter (fst #> map_option (mk_CONSTRAINT_rl ctxt))
                   |> Tactic.build_net
 
 
@@ -941,7 +932,7 @@ ML {*
                     pretty_constraint ctxt c
                   ] |> Pretty.string_of |> tracing
 
-                  val rl = mk_CONSTRAINT_rl thy c 
+                  val rl = mk_CONSTRAINT_rl ctxt c 
                      |> Drule.zero_var_indexes
                   val res = (SOLVED' (rtac rl 
                       THEN_ALL_NEW (REPEAT_ALL_NEW (resolve_from_net_tac ctxt net)))
@@ -966,10 +957,9 @@ ML {*
 
 
     fun solve_step_tac ctxt = let
-      val thy = Proof_Context.theory_of ctxt
       val pairs = thm_pairsD.get ctxt
       val net = pairs
-        |> map_filter (fst #> map_option (mk_CONSTRAINT_rl thy))
+        |> map_filter (fst #> map_option (mk_CONSTRAINT_rl ctxt))
         |> Tactic.build_net
     in 
       resolve_from_net_tac ctxt net
